src/program_proof/mvcc/examples_proof.v
@@ -1,0 +1,56 @@
+(* Import definitions/theorems of the Perennial framework with the disk FFI. *)
+From Perennial.program_proof Require Export disk_prelude.
+(* Import Coq model of our Goose program. *)
+From Goose.github_com.mit_pdos.go_mvcc Require Import examples.
+From Perennial.program_proof.mvcc Require Import txn_proof.
+
+Section heap.
+Context `{!heapGS Σ, !mvcc_ghostG Σ}.
+
+Theorem wp_Example1 txn γ :
+  {{{ is_txn_uninit txn γ }}}
+    Example1 #txn
+  {{{ (total : u64), RET #total; ⌜(int.Z total) = 10⌝ }}}.
+Proof.
+  iIntros (Φ) "Htxn HΦ".
+  wp_call.
+  wp_apply (wp_txn__Begin with "Htxn").
+  iIntros "Htxn".
+  wp_pures.
+  (* Read key 0 *)
+  wp_apply (wp_txn__Get with "Htxn").
+  iIntros (v ok) "Hget".
+  unfold get_spec.
+  rewrite lookup_empty.
+  iDestruct "Hget" as (v0) "[Htxn ->]".
+  wp_pures.
+  (* Read key 2 *)
+  wp_apply (wp_txn__Get with "Htxn").
+  iIntros (v ok') "Hget".
+  unfold get_spec.
+  rewrite lookup_empty.
+  replace (<[(U64 0):=v0]> _ !! (U64 2)) with (None : option u64); last first.
+  { symmetry. by rewrite lookup_insert_None. }
+  iDestruct "Hget" as (v2) "[Htxn ->]".
+  wp_pures.
+  iApply "HΦ".
+  iModIntro.
+  iDestruct (db_consistent with "Htxn") as (dbmap) "%Hdbmap".
+  iPureIntro.
+  destruct Hdbmap as [(v0' & v2' & (Hv0' & Hv2' & HC)) Hsubset].
+  assert (Hv0 : dbmap !! (U64 0) = Some v0).
+  { eapply lookup_weaken; last eauto.
+    rewrite lookup_insert_ne; last done.
+    apply lookup_insert.
+  }
+  assert (Hv2 : dbmap !! (U64 2) = Some v2).
+  { eapply lookup_weaken; last eauto.
+    apply lookup_insert.
+  }
+  rewrite Hv0 in Hv0'. inversion Hv0'.
+  rewrite Hv2 in Hv2'. inversion Hv2'.
+  subst.
+  word.
+Qed.
+
+End heap.
