src/program_proof/mvcc/index_proof.v
@@ -1,0 +1,20 @@
+(* Import definitions/theorems of the Perennial framework with the disk FFI. *)
+From Perennial.program_proof Require Export disk_prelude.
+(* Import Coq model of our Goose program. *)
+From Goose.github_com.mit_pdos.go_mvcc Require Import index.
+From Perennial.program_proof.mvcc Require Import mvcc_ghost tuple_proof.
+
+Section heap.
+Context `{!heapGS Σ, !mvcc_ghostG Σ}.
+
+Definition is_index (idx : loc) (γ : mvcc_names) : iProp Σ := True.
+
+Theorem wp_index__GetTuple idx (key : u64) γ :
+  is_index idx γ -∗
+  {{{ True }}}
+    Index__GetTuple #idx #key
+  {{{ (tuple : loc), RET #tuple; is_tuple tuple key γ }}}.
+Proof.
+Admitted.
+  
+End heap.
