src/program_proof/mvcc/mvcc_ghost.v
@@ -1,0 +1,64 @@
+From Perennial.program_proof Require Import disk_prelude.
+From iris.base_logic.lib Require Import ghost_map.
+From iris.algebra Require Import dfrac_agree.
+
+Local Definition key_fixedR := gmapR u64 (dfrac_agreeR (leibnizO nat)).
+
+Class mvcc_ghostG Σ :=
+  {
+    (*
+    mvcc_ghost_dbmaps :> ghost_mapG Σ (nat * u64) u64;
+    mvcc_ghost_key_fixed :> inG Σ key_fixedR;
+    *)
+    (* XXX: remove this *)
+    mvcc_ghost_versG :> ghost_varG Σ (list (u64 * u64 * u64))
+  }.
+
+Definition mvcc_ghostΣ := #[(*ghost_mapΣ (nat * u64) u64; GFunctor key_fixedR;*) (* XXX *) ghost_varΣ (list (u64 * u64 * u64))].
+
+Global Instance subG_mvcc_ghostG {Σ} :
+  subG mvcc_ghostΣ Σ → mvcc_ghostG Σ.
+Proof. solve_inG. Qed.
+
+Record mvcc_names :=
+  {
+    (*
+    mvcc_dbmaps : gname;
+    mvcc_fixed : gname;
+    *)
+    (* XXX *)
+    tuple_vers_gn : gname
+  }.
+
+Section definitions.
+Context `{!heapGS Σ, !mvcc_ghostG Σ}.
+
+(* Definition tid_sentinel : nat := 18446744073709551615%nat. *)
+
+Definition mvccN := nroot .@ "mvcc_inv".
+
+
+(* The following points-to facts are defined in terms of the underlying CC resources. *)
+Definition view_ptsto (k v : u64) : iProp Σ := True.
+Definition mods_token (k : u64) : iProp Σ := True.
+
+Theorem view_ptsto_agree (k v v' : u64) :
+  view_ptsto k v -∗ view_ptsto k v' -∗ ⌜v = v'⌝.
+Admitted.
+
+(*
+Definition fixed_ptsto γ (q : Qp) (key : u64) (fixed : nat) : iProp Σ :=
+  own γ.(mvcc_fixed) {[key := to_dfrac_agree (DfracOwn q) (fixed : (leibnizO _))]}.
+
+Definition db_ptsto γ (dq : dfrac) (ts : nat) (key : u64) (val : u64) : iProp Σ :=
+  (ts, key) ↪[γ.(mvcc_dbmaps)]{dq} val.
+
+Definition mvcc_invariant γ : iProp Σ :=
+  ∃ dbmaps,
+    ghost_map_auth γ.(mvcc_dbmaps) 1 dbmaps.
+
+Definition mvcc_inv γ : iProp Σ :=
+  inv mvccN (mvcc_invariant γ).
+*)
+
+End definitions.
