src/program_proof/mvcc/txn_proof.v
@@ -1,0 +1,425 @@
+(* Import definitions/theorems of the Perennial framework with the disk FFI. *)
+From Perennial.program_proof Require Export disk_prelude.
+(* Import Coq model of our Goose program. *)
+From Goose.github_com.mit_pdos.go_mvcc Require Import txn.
+From Perennial.program_proof.mvcc Require Import mvcc_ghost index_proof tuple_proof.
+
+Section heap.
+Context `{!heapGS Σ, !mvcc_ghostG Σ}.
+
+(**
+ * 1. A txn is exposed to the client as two maps:
+ *    a) `view`: one read-only map that represents the contents of the database on which
+ *       the consistency predicate can be deduced,
+ *    b) `mods`: another map that represents the updates made by the txn.
+ * 2. `is_txn` connects the two maps with the following two kinds of resources:
+ *    a) `view_ptsto k v` says that value `v` is stored at location `k`,
+ *    b) `mods_token k` allows the txn to update `k`.
+ * 3. These resources are defined by the underlying concurrency control protocol.
+ *    They are granted on get and put, and returned on commit and abort.
+ *    This roughly matches the idea of "reduction to two-phase locking".
+ * 4. The spec of begin/commit/abort/get/put mentions only the two maps (`view` and `mods`),
+ *    not the points-to facts (i.e., they are hidden behind `is_txn`).
+ *    The client should be able to deduce the consistency predicate without expanding `is_txn`.
+ * 5. The database invariant consists of:
+ *    a) the authoritative element that represents the entire database,
+ *    b) the consistency predicate,
+ *    c) something that can give the client a proof that the txn actually executes.
+ *)
+
+(* Client-defined consistency predicate. *)
+Definition C (m : gmap u64 u64) :=
+  ∃ v0 v2,
+    (m !! (U64 0) = Some v0) ∧ (m !! (U64 2) = Some v2) ∧
+    (int.Z v0) + (int.Z v2) = 10.
+
+(* `dbmap` is a map representing the entire database. *)
+(*
+Definition dbinv dbmap := ●dbmap ∗ (C dbmap) ∗ ●log.
+ *)
+
+Definition wrent_to_val (x : u64 * u64 * loc) :=
+  (#x.1.1, (#x.1.2, (#x.2, #())))%V.
+
+Definition own_txnmgr (txnmgr : loc) : iProp Σ := 
+  ∃ (sidcur : u64) (sites : Slice.t)
+    (* TODO: make `sites` a slice of pointers to `TxnSite` in the implementation. *)
+    (sitesL : list loc),
+    "Hsidcur" ∷ txnmgr ↦[TxnMgr :: "sidCur"] #sidcur ∗
+    "Hsites" ∷ txnmgr ↦[TxnMgr :: "sites"] (to_val sites) ∗
+    "HwsetL" ∷ slice.is_slice sites (structTy TxnSite) 1 (to_val <$> sitesL) ∗
+    "_" ∷ True.
+
+Definition is_txnmgr (txnmgr : loc) γ : iProp Σ := 
+  ∃ (latch : loc) (sidcur : u64) (sites : Slice.t) (idx gc : loc)
+    (sitesL : list loc),
+    "#Hlatch" ∷ readonly (txnmgr ↦[TxnMgr :: "latch"] #latch) ∗
+    "#Hlock" ∷ is_lock mvccN #latch (own_txnmgr txnmgr) ∗
+    (* TODO: `is_idx` and `is_gc` *)
+    "#Hidx" ∷ readonly (txnmgr ↦[TxnMgr :: "idx"] #idx) ∗
+    "#HidxRI" ∷ is_index idx γ ∗
+    "#Hgc" ∷ readonly (txnmgr ↦[TxnMgr :: "gc"] #gc) ∗
+    "_" ∷ True.
+
+Definition is_txn_impl (txn : loc) (view mods : gmap u64 u64) γ : iProp Σ :=
+  ∃ (tid sid : u64) (wset : Slice.t) (idx txnmgr : loc)
+    (wsetL : list (u64 * u64 * loc)),
+    "Htid" ∷ txn ↦[Txn :: "tid"] #tid ∗
+    "Hsid" ∷ txn ↦[Txn :: "sid"] #sid ∗
+    "Hwset" ∷ txn ↦[Txn :: "wset"] (to_val wset) ∗
+    "HwsetL" ∷ slice.is_slice wset (structTy WrEnt) 1 (wrent_to_val <$> wsetL) ∗
+    "%HwsetLND" ∷ ⌜NoDup (fst <$> wsetL).*1⌝ (* keys are unique *) ∗
+    "%Hmods_wsetL" ∷ ⌜mods = (list_to_map (fst <$> wsetL))⌝ ∗
+    "#Hidx" ∷ readonly (txn ↦[Txn :: "idx"] #idx) ∗
+    "#HidxRI" ∷ is_index idx γ ∗
+    "Htxnmgr" ∷ txn ↦[Txn :: "txnMgr"] #txnmgr ∗
+    "HtxnmgrRI" ∷ is_txnmgr txnmgr γ ∗
+    "_" ∷ True.
+
+Definition is_txn (txn : loc) (view mods : gmap u64 u64) γ : iProp Σ :=
+  "%Hsubset" ∷ ⌜dom (gset u64) mods ⊆ dom (gset u64) view⌝ ∗
+  (* TODO: separating permissions from values? *)
+  "Hmods" ∷ ([∗ map] k ↦ _ ∈ mods, mods_token k) ∗
+  "Hview" ∷ ([∗ map] k ↦ v ∈ view, view_ptsto k v) ∗
+  "Himpl" ∷ is_txn_impl txn view mods γ.
+
+Definition is_txn_uninit (txn : loc) γ : iProp Σ := 
+  ∃ (tid sid : u64) (wset : Slice.t) (idx txnmgr : loc)
+    (wsetL : list (u64 * u64 * loc)),
+    "Htid" ∷ txn ↦[Txn :: "tid"] #tid ∗
+    "Hsid" ∷ txn ↦[Txn :: "sid"] #sid ∗
+    "Hwset" ∷ txn ↦[Txn :: "wset"] (to_val wset) ∗
+    "HwsetL" ∷ slice.is_slice wset (structTy WrEnt) 1 (wrent_to_val <$> wsetL) ∗
+    "#Hidx" ∷ readonly (txn ↦[Txn :: "idx"] #idx) ∗
+    "#HidxRI" ∷ is_index idx γ ∗
+    "Htxnmgr" ∷ txn ↦[Txn :: "txnMgr"] #txnmgr ∗
+    "HtxnmgrRI" ∷ is_txnmgr txnmgr γ ∗
+    "_" ∷ True.
+
+Definition is_txnsite (txnsite : loc) : iProp Σ := 
+  ∃ (latch : loc) (tidlast : u64) (tidsactive : Slice.t)
+    (tidsactiveL : list u64),
+    "#Hlatch" ∷ readonly (txnsite ↦[TxnSite :: "latch"] #latch) ∗
+    "Htidlast" ∷ txnsite ↦[TxnSite :: "tidLast"] #tidlast ∗
+    "Hwset" ∷ txnsite ↦[TxnSite :: "tidsActive"] (to_val tidsactive) ∗
+    "HwsetL" ∷ typed_slice.is_slice tidsactive uint64T 1 tidsactiveL ∗
+    "_" ∷ True.
+
+Local Hint Extern 1 (environments.envs_entails _ (is_txn _ _ _ _)) => unfold is_txn : core.
+Local Hint Extern 1 (environments.envs_entails _ (is_txn_impl _ _ _ _)) => unfold is_txn_impl : core.
+
+(**
+ * Extensions of a map are supersets of the map that we logically have
+ * access to, but physically (i.e., the program) does not.
+ *)
+
+(* The client can use this theorem to deduce `C` without expanding the definition of `is_txn`. *)
+Theorem db_consistent txn view mods γ :
+  ⊢ is_txn txn view mods γ →
+    ∃ dbmap, ⌜C dbmap ∧ view ⊆ dbmap⌝.
+Proof.
+  iIntros "Htxn".
+  (* 1. Open `dbinv`. *)
+  (* 2. Apply the agree rule to deduce that `view` is a subset of `dbmap`. *)
+  (* 3. Deduce that `C` holds on `view`. *)
+Admitted.
+
+(*
+{{{ True }}} wp_txn__New {{{ is_txn_uninit txn }}}
+*)
+
+(*****************************************************************)
+(* func genTID(sid uint64) uint64                                *)
+(*****************************************************************)
+Theorem wp_genTID (sid : u64) :
+  {{{ True }}}
+    genTID #sid
+  {{{ (tid : u64), RET #tid; True }}}.
+Proof.
+  iIntros (Φ) "Hpre HΦ".
+  wp_call.
+
+  (***********************************************************)
+  (* var tid uint64                                          *)
+  (***********************************************************)
+  wp_apply wp_ref_of_zero; first done.
+  iIntros (tid) "Htid".
+  wp_pures.
+  wp_call.
+
+  (***********************************************************)
+  (* tid = tsc.GetTSC()                                      *)
+  (***********************************************************)
+  wp_apply wp_ArbitraryInt.
+  iIntros (tsc) "_".
+
+  (***********************************************************)
+  (* tid = (tid & ^(config.N_TXN_SITES - 1)) + sid           *)
+  (***********************************************************)
+  wp_store.
+  wp_load.
+  wp_store.
+  wp_load.
+
+  (***********************************************************)
+  (* return tid                                              *) 
+  (***********************************************************)
+  iApply "HΦ".
+  done.
+Qed.
+
+Theorem wp_txnMgr__activate (txnmgr : loc) (sid : u64) γ :
+  {{{ is_txnmgr txnmgr γ }}}
+    TxnMgr__activate #txnmgr #sid
+  {{{ (tid : u64), RET #tid; is_txnmgr txnmgr γ }}}.
+Proof.
+  iIntros (Φ) "Htxnmgr HΦ".
+  iNamed "Htxnmgr".
+  wp_call.
+Admitted.
+
+(*****************************************************************)
+(* func (txn *Txn) Begin()                                       *)
+(*****************************************************************)
+Theorem wp_txn__Begin txn γ :
+  {{{ is_txn_uninit txn γ }}}
+    Txn__Begin #txn
+  {{{ RET #(); is_txn txn ∅ ∅ γ }}}.
+Proof.
+  iIntros (Φ) "Htxn HΦ".
+  iNamed "Htxn".
+  wp_call.
+  
+  (***********************************************************)
+  (* tid := txn.txnMgr.activate(txn.sid)                     *)
+  (***********************************************************)
+  wp_loadField.
+  wp_loadField.
+  wp_apply (wp_txnMgr__activate with "HtxnmgrRI").
+  rename tid into tid_tmp.
+  iIntros (tid) "HtxnmgrRI".
+
+  (***********************************************************)
+  (* txn.tid = tid                                           *)
+  (***********************************************************)
+  wp_pures.
+  wp_storeField.
+  
+  (***********************************************************)
+  (* txn.wset = txn.wset[:0]                                 *)
+  (***********************************************************)
+  wp_loadField.
+  wp_apply (wp_SliceTake); first word.
+  wp_apply (wp_storeField with "Hwset"); first eauto.
+  iIntros "Hwset".
+  wp_pures.
+  
+  iApply "HΦ".
+  iModIntro.
+  rewrite /is_txn.
+  do 3 (iSplitR; first eauto).
+  iExists _, _, _, _, _, [].
+  iFrame "# ∗".
+  repeat rewrite fmap_nil.
+  iDestruct (is_slice_take_cap _ _ _ (U64 0) with "HwsetL") as "H"; first word.
+  iSplit; first done.
+  iPureIntro.
+  split; auto using NoDup_nil_2.
+Qed.
+
+(*****************************************************************)
+(* func matchLocalWrites(key uint64, wset []WrEnt) (uint64, bool)*)
+(*****************************************************************)
+Local Lemma wp_matchLocalWrites (key : u64) (wset : Slice.t) (wsetL : list (u64 * u64 * loc)) :
+  {{{ slice.is_slice wset (structTy WrEnt) 1 (wrent_to_val <$> wsetL) }}}
+    matchLocalWrites #key (to_val wset)
+  {{{ (pos : u64) (found : bool), RET (#pos, #found);
+        slice.is_slice wset (structTy WrEnt) 1 (wrent_to_val <$> wsetL) ∗
+        ⌜(found = false ∧ key ∉ wsetL.*1.*1) ∨
+         (found = true ∧ ∃ went, wsetL !! (int.nat pos) = Some went ∧ went.1.1 = key)⌝
+  }}}.
+Proof.
+  (***********************************************************)
+  (* var idx uint64 = 0                                      *)
+  (* var found bool = false                                  *)
+  (* for {                                                   *)
+  (*   if idx >= uint64(len(wset)) {                         *)
+  (*     break                                               *)
+  (*   }                                                     *)
+  (*   if key == wset[idx].key {                             *)
+  (*     found = true                                        *)
+  (*     break                                               *)
+  (*   }                                                     *)
+  (*   idx++                                                 *)
+  (* }                                                       *)
+  (* return idx, found                                       *)
+  (***********************************************************)
+Admitted.
+
+Definition get_spec txn view mods k v γ : iProp Σ :=
+  match view !! k, mods !! k with
+  (* `k` has not been read or written. *)
+  | None, None => ∃ v', is_txn txn (<[k := v']> view) mods γ ∧ ⌜v = v'⌝
+  (* `k` has been read, but not written. *)
+  | Some vr, None => is_txn txn view mods γ ∧ ⌜v = vr⌝
+  (* `k` has been written. *)
+  | _, Some vw => is_txn txn view mods γ ∧ ⌜v = vw⌝
+  end.
+
+(*****************************************************************)
+(* func (txn *Txn) Get(key uint64) (uint64, bool)                *)
+(*****************************************************************)
+Theorem wp_txn__Get txn (k : u64) (view mods : gmap u64 u64) γ :
+  {{{ is_txn txn view mods γ }}}
+    Txn__Get #txn #k
+  {{{ (v : u64) (ok : bool), RET (#v, #ok); get_spec txn view mods k v γ }}}.
+Proof.
+  iIntros (Φ) "Htxn HΦ".
+  iNamed "Htxn".
+  iNamed "Himpl".
+  wp_call.
+
+  (***********************************************************)
+  (* pos, found := matchLocalWrites(key, txn.wset)           *)
+  (***********************************************************)
+  wp_loadField.
+  wp_apply (wp_matchLocalWrites with "HwsetL").
+  iIntros (pos found) "[HwsetL %Hmatch]".
+  wp_pures.
+  
+  (***********************************************************)
+  (* if found {                                              *)
+  (*   val := txn.wset[pos].val                              *)
+  (*   return val, true                                      *)
+  (* }                                                       *)
+  (***********************************************************)
+  iDestruct (slice.is_slice_small_acc with "HwsetL") as "[HwsetL HwsetL_close]".
+  wp_if_destruct.
+  { wp_loadField.
+    destruct Hmatch as [[contra _] | [_ [went [Hlookup Hkey]]]]; first congruence.
+    wp_apply (wp_SliceGet with "[HwsetL]").
+    { iFrame.
+      iPureIntro.
+      rewrite list_lookup_fmap.
+      by rewrite Hlookup.
+    }
+    iIntros "[HwsetL %Hwent]".
+    wp_pures.
+    iApply "HΦ".
+    iModIntro.
+    rewrite /get_spec.
+    (* Proving the third case of `get_spec` (write set hit). *)
+    assert (HmodsSome : ∃ vm, mods !! k = Some vm).
+    { exists went.1.2.
+      rewrite Hmods_wsetL.
+      rewrite -elem_of_list_to_map; last auto.
+      apply elem_of_list_fmap_1_alt with went.
+      { by apply elem_of_list_lookup_2 with (int.nat pos). }
+      { rewrite -Hkey. auto using surjective_pairing. }
+    }
+    destruct HmodsSome as [vm HmodsSome].
+    assert (HviewSome : ∃ vv, view !! k = Some vv).
+    { apply elem_of_dom_2 in HmodsSome as Hinmods.
+      (* Q: why doesn't the following work? *)
+      (* destruct (elem_of_weaken _ _ _ Hinmods Hsubset). *)
+      assert (Hinview : k ∈ dom (gset u64) view).
+      { by apply elem_of_weaken with (dom (gset u64) mods). }
+      by apply elem_of_dom in Hinview.
+    }
+    destruct HviewSome as [vv HviewSome].
+    rewrite HviewSome.
+    rewrite HmodsSome.
+    iSplit; last first.
+    { iPureIntro.
+      rewrite Hmods_wsetL in HmodsSome.
+      apply elem_of_list_lookup_2 in Hlookup.
+      apply (elem_of_list_fmap_1 fst) in Hlookup.
+      rewrite (surjective_pairing went.1) in Hlookup.
+      rewrite Hkey in Hlookup.
+      apply elem_of_list_to_map_1 in Hlookup; last auto.
+      rewrite Hlookup in HmodsSome.
+      by inversion HmodsSome.
+    }
+    iDestruct ("HwsetL_close" with "HwsetL") as "HwsetL".
+    eauto 20 with iFrame.
+  }
+
+  (***********************************************************)
+  (* idx := txn.idx                                          *)
+  (* tuple := idx.GetTuple(key)                              *)
+  (* valTuple, foundTuple := tuple.ReadVersion(txn.tid)      *)
+  (* return valTuple, foundTuple                             *)
+  (***********************************************************)
+  iDestruct ("HwsetL_close" with "HwsetL") as "HwsetL".
+  wp_loadField.
+  wp_pures.
+  wp_apply (wp_index__GetTuple with "HidxRI").
+  iIntros (tuple) "#HtupleRI".
+  wp_pures.
+  wp_loadField.
+  wp_apply (wp_tuple__ReadVersion with "HtupleRI").
+  clear Heqb found.
+  iIntros (val found) "Hview_ptsto'".
+  wp_pures.
+  iApply "HΦ".
+  iModIntro.
+  rewrite /get_spec.
+  assert (HmodsNone : mods !! k = None).
+  { destruct Hmatch as [[_ Hnotin] | [contra _]]; last congruence.
+    rewrite Hmods_wsetL.
+    by apply not_elem_of_list_to_map.
+  }
+  rewrite HmodsNone.
+  destruct (view !! k) eqn:Eqlookup.
+  { (* Proving the second case of `get_spec` (write set misses / non-first read). *)
+    iDestruct (big_sepM_lookup_acc _ view k u with "[Hview]") as "[Hview_ptsto Hview_close]"; [auto | auto |].
+    iDestruct (view_ptsto_agree with "Hview_ptsto Hview_ptsto'") as %->.
+    iDestruct ("Hview_close" with "Hview_ptsto") as "Hview".
+    iSplit; last done.
+    eauto 20 with iFrame.
+  }
+  { (* Proving the first case of `get_spec` (write set misses / first read). *)
+    iExists val.
+    iSplit; last done.
+    rewrite /is_txn.
+    iSplit.
+    { iPureIntro.
+      rewrite dom_insert.
+      set_solver.
+    }
+    iFrame "Hmods".
+    iSplitL "Hview Hview_ptsto'".
+    { iApply big_sepM_insert; done. }
+    eauto 20 with iFrame.
+  }
+  (* Qed. *)
+  (* Error: The following section variable is used but not declared: mvcc_ghostG0 *)
+Admitted.
+
+Definition put_spec txn view mods k v γ : iProp Σ :=
+  match view !! k, mods !! k with
+  (* `k` has not been read or written; note that `v'` is not tied to any program variable. *)
+  | None, None => ∃ v', is_txn txn (<[k := v']> view) (<[k := v]> mods) γ
+  (* `k` has been read or written. *)
+  | _, _ => is_txn txn view (<[k := v]> mods) γ
+  end.
+
+Theorem wp_txn__Put txn (k : u64) (v : u64) (view mods : gmap u64 u64) γ :
+  {{{ is_txn txn view mods γ }}}
+    Txn__Put #txn #k #v
+  {{{ (ok : bool), RET #ok; put_spec txn view mods k v γ }}}.
+Proof.
+  iIntros (Φ) "Htxn HΦ".
+  iNamed "Htxn".
+  iNamed "Himpl".
+  wp_call.
+Admitted.
+
+(* The client is responsible for proving C holds on all the updated extensions of `view`. *)
+Theorem wp_txn__Commit txn view mods γ :
+  {{{ ∀ dbmap, ⌜view ⊆ dbmap → C dbmap → C (mods ∪ dbmap)⌝ ∗ is_txn txn view mods γ }}}
+    Txn__Commit #txn
+  {{{ RET #(); is_txn_uninit txn γ (* * sth about log *) }}}.
+Admitted.
+
+End heap.
